src/impl/TLS13.Handshake.ByteDriver.External.fsti
@@ -7,49 +7,57 @@ open Pulse.Lib.Pervasives
 module IO = TLS13.IO
 module U8 = FStar.UInt8
 
+type progress =
+  | ExpectEncryptedExtensions
+  | ExpectCertificate
+  | ExpectCertificateVerify
+  | ExpectFinished
+  | Complete
+
 val context : Type0
-val is_context: context -> slprop
+val is_context: context -> progress -> slprop
 
 fn reset_encrypted_handshake (ctx: context)
-  requires is_context ctx
-  ensures is_context ctx
+  requires is_context ctx 'p
+  ensures is_context ctx ExpectEncryptedExtensions
 
 fn read_next_encrypted_handshake_record (ctx: context) (ch: IO.channel)
-  requires is_context ctx ** IO.is_channel ch
+  requires is_context ctx 'p ** IO.is_channel ch
   returns ok: bool
-  ensures is_context ctx ** IO.is_channel ch
+  ensures is_context ctx 'p ** IO.is_channel ch
 
 fn pending_handshake_message_complete (ctx: context)
-  requires is_context ctx
+  requires is_context ctx 'p
   returns complete: bool
-  ensures is_context ctx
+  ensures is_context ctx 'p
 
 fn pending_handshake_message_type (ctx: context)
-  requires is_context ctx
+  requires is_context ctx 'p
   returns msg_type: U8.t
-  ensures is_context ctx
+  ensures is_context ctx 'p
 
 fn accept_encrypted_extensions (ctx: context)
-  requires is_context ctx
+  requires is_context ctx ExpectEncryptedExtensions
   returns ok: bool
-  ensures is_context ctx
+  ensures is_context ctx (if ok then ExpectCertificate else ExpectEncryptedExtensions)
 
 fn accept_certificate (ctx: context)
-  requires is_context ctx
+  requires is_context ctx ExpectCertificate
   returns ok: bool
-  ensures is_context ctx
+  ensures is_context ctx (if ok then ExpectCertificateVerify else ExpectCertificate)
 
 fn accept_certificate_verify (ctx: context)
-  requires is_context ctx
+  requires is_context ctx ExpectCertificateVerify
   returns ok: bool
-  ensures is_context ctx
+  ensures is_context ctx (if ok then ExpectFinished else ExpectCertificateVerify)
 
 fn accept_finished (ctx: context)
-  requires is_context ctx
+  requires is_context ctx ExpectFinished
   returns ok: bool
-  ensures is_context ctx
+  ensures is_context ctx (if ok then Complete else ExpectFinished)
 
 fn encrypted_handshake_complete (ctx: context)
-  requires is_context ctx
+  requires is_context ctx 'p
   returns done: bool
-  ensures is_context ctx
+  ensures is_context ctx 'p **
+          pure (done ==> 'p == Complete)
